src/Memory.lean
@@ -1,4 +1,4 @@
-import Utility tactic 
+import Utility tactic data.nat.basic
 
 def mem_spec {α : Type} (D : stream α) (S : signal) (M : stream α) : Prop :=
   ∀ t : ℕ,
@@ -13,44 +13,69 @@ def almost_eq' {α : Type} (N M : stream α) : Prop :=
   ∀ (t : ℕ),
     (N t = M t) → N (t+1) = M (t+1)
 
-lemma almost_eq_equiv {α : Type} (N M : stream α) : almost_eq N M ↔ almost_eq' N M :=
+lemma help {t' t n: nat} (h: t' > t) (hh: t' - t = n): t' = t + n :=
   begin
-    unfold almost_eq almost_eq',
-    split,
-    {
-      intros h t,
-      specialize h t,
-      intros h₁,
-      apply h,
-      {
-        exact h₁,
-      },
-      {
-        simp,
-      }
-    },
-    {
-      intros h t,
-      specialize h t,
-      intros h₁ t' ht',
-      specialize h,
-      
-      cases t',
-      {
-        finish,
-      },
-      {
-        cases ht' with,
-        {
-          finish,
-        },
-        {
-          finish,
-        }
-        
-      }
-    }
+    rw ←hh,
+    rw nat.add_sub_of_le,
+    exact le_of_lt h,
   end
+
+lemma almost_eq_equiv {α : Type} (N M : stream α) : almost_eq N M ↔
+almost_eq' N M :=
+   begin
+     unfold almost_eq almost_eq',
+     split,
+     {
+       intros h t,
+       specialize h t,
+       intros h₁,
+       apply h,
+       {
+         exact h₁,
+       },
+       {
+         simp,
+       }
+     },
+     {
+       intros h t h₁ t' h₂,
+       -- We have t' > t, so take the difference (dt)
+       generalize hhh: t' - t = dt,
+       destruct dt; intros; rw a at hhh,
+       {
+         -- Suppose dt = 0, then we can close the goal
+         rw (help h₂ hhh),
+         simp, tauto,
+       },
+       {
+         -- Suppose dt > 0, then do a strong induction
+         revert t',
+         apply (nat.strong_induction_on n); intros n_1 IH; intros,
+         destruct n_1; intros,
+         {
+           -- Suppose dt = 1
+           rw a_1 at hhh,
+           rw (help h₂ hhh),
+           apply h, tauto,
+         },
+         {
+           -- Otherwise
+           rw (help h₂ hhh),
+           apply h, simp,
+           apply (IH n_2),
+           {
+            rw a_1,
+            exact nat.lt_succ_self _,
+           },
+           repeat{
+            rw a_1,
+            simp,
+           },
+         }
+       }
+     }
+   end
+
 
 theorem mem_spec_almost_unique {α : Type} : ∀ (D : stream α) (S : signal) (M : stream α),
   mem_spec D S M → ∀(N : stream α), mem_spec D S N → almost_eq N M :=
@@ -82,56 +107,30 @@ theorem mem_spec_almost_unique {α : Type} : ∀ (D : stream α) (S : signal) (M
     }
   end
 
-def mem_imp (I: bool) (D S: signal) : signal
-  | nat.zero := I
-  | (nat.succ y) := if S y = tt then D y 
-                    else mem_imp y
 
-def mem_n_imp {n : ℕ} (I : array n bool) (D : sig_n n) (S : signal) : sig_n n
+def mem_imp {α : Type} (I : α) (D : stream α) (S : signal) : stream α
   | nat.zero := I
   | (nat.succ y) := if S y = tt then D y
-                    else mem_n_imp y
+                    else mem_imp y
 
-theorem mem_correct : ∀ (D S : signal), ∀ (I : bool),
-  mem_spec D S (mem_imp I D S) :=
-  begin
-    intros D S I,
-    unfold mem_spec,
-    intro t,
-    split,
-    {
-      intros h,
-      unfold mem_imp,
-      rw if_pos,
-      exact h,
-    },
-    {
-      intros h,
-      unfold mem_imp,
-      rw if_neg,
-      simp,
-      exact h,
-    }
-  end
 
-theorem mem_n_correct {n : ℕ} : ∀ (D : sig_n n) (S: signal), ∀ (I : array n bool),
-  mem_spec D S (mem_n_imp (I) D S) :=
+theorem mem_correct {α : Type} : ∀ (D : stream α) (S: signal), ∀ (I : α),
+  mem_spec D S (mem_imp (I) D S) :=
   begin
     unfold mem_spec,
     intros,
     split,
     {
       intros h,
-      unfold mem_n_imp,
+      unfold mem_imp,
       rw if_pos,
       exact h,
     },
     {
       intros h,
-      unfold mem_n_imp,
+      unfold mem_imp,
       rw if_neg,
       simp,
       exact h,
     }
   end
-
